Veritas.Verifier.Correctness.fst
@@ -1,0 +1,94 @@
+module Veritas.Verifier.Correctness
+
+open FStar.Seq
+open Veritas.Key
+open Veritas.MultiSetHash
+open Veritas.Record
+open Veritas.Verifier
+open Veritas.SeqAux
+
+//Allow the solver to unroll recursive functions at most once (fuel)
+//Allow the solver to invert inductive definitions at most once (ifuel)
+#push-options "--max_fuel 1 --max_ifuel 1 --initial_fuel 1 --initial_ifuel 1"
+
+(* Does the verifier return Valid (success) for this log *)
+let verifiable (#p:pos) (l:vlog) = Valid? (verifier #p l)
+
+(* Refinement type of logs that are verifiable *)
+type verifiable_log (#p:pos) = l:vlog{verifiable #p l}
+
+(* If a log is verifiable, then each prefix of the log is also verifiable *)
+let rec lemma_verifiable_implies_prefix_verifiable (#p:pos) (l:verifiable_log #p) (i:nat{i <= length l}):
+  Lemma (requires (True))
+        (ensures (verifiable #p (prefix l i)))
+        (decreases (length l)) =
+  let n = length l in
+  if n = 0 then ()
+  else if i = n then ()
+  else
+    lemma_verifiable_implies_prefix_verifiable #p (prefix l (n - 1)) i
+
+(* TODO: #p seems to prevent the use of SMTPat in lemma above *)
+let vprefix (#p:pos) (l:verifiable_log #p) (i:nat{i <= length l}): 
+  l':(verifiable_log #p){l' = prefix l i} = 
+  lemma_verifiable_implies_prefix_verifiable l i;
+  prefix l i
+
+(* is this a thread-local operation *)
+let is_thread_op (e:vlog_entry_g) = TOp? e
+
+(* is the operator at index i a thread-local op *)
+let is_thread_op_idx (l:vlog) (i:vl_index l) = 
+  is_thread_op (index l i)
+
+(* thread id of a thread-local op *)
+let thread_id_of (e:vlog_entry_g {is_thread_op e}) = 
+  TOp?.tid e
+
+let thread_id_of_idx (l:vlog) (i:vl_index l{is_thread_op_idx l i}) = 
+  thread_id_of (index l i)
+
+(* thread id of every thread-local op < p (verifier parallelism) *)
+let lemma_thread_id_valid (#p:pos) 
+                          (l:verifiable_log #p) 
+                          (i:vl_index l {is_thread_op_idx l i})
+  : Lemma (thread_id_of_idx l i < p) = 
+  let l' = vprefix l i in
+  let l'' = vprefix l (i + 1) in
+  ()
+         
+(* 
+ * we associate a timestamp to every thread-local op based on the 
+ * thread clock after the completion of the operation 
+ *)
+let op_clock (#p:pos) 
+             (l:verifiable_log #p) 
+             (i:vl_index l {is_thread_op_idx l i}): timestamp = 
+ let l' = vprefix l (i + 1) in
+ let vs = verifier #p l' in
+ let ti = thread_id_of_idx l i in
+ lemma_thread_id_valid l i;
+ thread_clock ti vs
+
+(* thread-local log: a log with only thread-local operations (no VerifyEpoch) *)
+type thread_local_log (l:vlog) = forall (i:vl_index l). {:pattern (is_thread_op_idx l i)} is_thread_op_idx l i
+
+type tl_log (#p:pos) = l:(verifiable_log #p){thread_local_log l}
+
+(* a thread-local log is clock-ordered is the clock of each operation is monotonically increasing *)
+type clock_ordered_log (#p:pos) (l:tl_log #p) = 
+  forall (i:vl_index l). i > 0 ==> (op_clock l i `ts_geq` op_clock l (i - 1))
+
+type co_log (#p:pos) = l:(tl_log #p){clock_ordered_log l}
+
+(* the key referenced by an log operation *)
+let key_of (e:vlog_entry) = 
+  match e with
+  | Get k _ -> k
+  | Put k _ -> k
+  | AddM r _ -> let (k,_) = r in k
+  | EvictM k _ -> k
+  | AddB r _ _ -> let (k,_) = r in k
+  | EvictB k _ -> k
+  | EvictBM k _ _ -> k
+
